Lamcalc.lean
@@ -9,3 +9,4 @@ import Lamcalc.Confluence
 import Lamcalc.Context
 import Lamcalc.Typed
 import Lamcalc.Weakening
+import Lamcalc.Substitution
