Lamcalc/Context.lean
@@ -4,10 +4,10 @@ abbrev Ctx := List Tm
 
 inductive Has : Ctx -> Var -> Tm -> Prop where
   | zero :
-    Has (a :: Γ) 0 a.[shift]
+    Has (a :: Γ) 0 a.[ren .succ]
   | succ :
     Has Γ x a ->
-    Has (b :: Γ) x.succ a.[shift]
+    Has (b :: Γ) x.succ a.[ren .succ]
 
 theorem has_sized : Has Γ x a -> x < Γ.length := by
   intro h
